Code/Reg_Exp_Prop.v
@@ -1,4 +1,13 @@
 (*Reg_Exp1=Reg_Exp2 wenn beide die gleiche Sprache beschreiben*)
+Require Import Reg_Exp.
+
+Lemma Reg_plus {A:Type} (e1 : @Reg_Exp A) :
+    Plus e1 e1  = e1.
+Proof.
+destruct Plus.
+-
+
+
 
 (*Die Gleichheit zwischen regulären Ausdrücken ist entscheidbar.*)
 
